Small_Step.thy
@@ -66,7 +66,7 @@ lemmas small_step_induct = small_step.induct[split_format(complete)]
 
 subsubsection{* Proof automation *}
 
-declare small_step.intros[simp,intro]
+declare small_step.intros[simp, intro]
 
 text{* Rule inversion: *}
 
@@ -75,6 +75,14 @@ inductive_cases SeqE[elim]: "(Some(c1;; c2), s) \<rightarrow> ct"
 inductive_cases IfE[elim!]: "(Some({P} IF b THEN c1 ELSE c2 FI), s) \<rightarrow> ct"
 inductive_cases WhileE[elim]: "(Some({P} WHILE b INV I DO c OD), s) \<rightarrow> ct"
 inductive_cases WaitE[elim]: "(Some({P} WAIT b END), s) \<rightarrow> ct"
+
+inductive_cases small_step_cases:
+    "(None,s) \<rightarrow> (c', s')"
+    "(Some ({P} x ::= a),s) \<rightarrow> (c', s')"
+    "(Some (c1;; c2), s) \<rightarrow> (c', s')"
+    "(Some ({P} IF b THEN c1 ELSE c2 FI), s) \<rightarrow> (c', s')"
+    "(Some ({P} WHILE b INV I DO c OD), s) \<rightarrow> (c', s')"
+    "(Some ({P} WAIT b END), s) \<rightarrow> (c', s')"
 
 
 text{* A simple property: *}
@@ -109,5 +117,74 @@ lemma tr_deterministic:
 apply(induction arbitrary: cs'' rule: small_step_tr.induct)
 apply blast+
 done
+
+lemma none_final:
+  assumes "(None, s) \<rightarrow>* (c, t)"
+  shows "c = None" and "s = t"
+proof -
+  from assms have "c = None \<and> s = t"
+  proof (induction "(None::(acom option), s)" "(c, t)" rule:star.induct)
+    case (step y)
+    from step.hyps(1) have "False"
+    by (induct "(None::(acom option),s)" y rule:small_step.induct)
+    thus ?case by auto
+  next
+    case refl
+    thus ?case by simp
+  qed
+  thus "c = None" and "s = t" by auto
+qed
+
+lemma final_det:
+  assumes "(c,s) \<rightarrow>* (None,t)"
+  and "(c,s) \<rightarrow>* (None, t')"
+  shows "t = t'"
+using assms
+proof (induct "(c,s)" "(None::(acom option), t)" arbitrary:c s rule:star.induct) 
+  case refl thus ?case by (simp add: none_final(2))  
+next
+  case step thus ?case using deterministic
+    by (metis (no_types, hide_lams) PairE none_final(2) star.simps)
+qed
+
+lemma star_seq2:
+  assumes "(Some c1, s) \<rightarrow>* (Some c1', s')"
+  shows "(Some(c1;; c2), s) \<rightarrow>* (Some(c1';; c2), s')"
+using assms
+proof(induction "(Some c1)" s "(Some c1')" "s'" arbitrary:c1 rule: star_induct[where r = small_step])
+  case refl thus ?case by simp
+next
+  case (step s con s' t)
+  from none_final step.hyps(1,2) obtain c where 1:"con = Some c" by fastforce
+  with step.hyps(3) have 2:"(Some c;; c2, s') \<rightarrow>* (Some c1';; c2, t)" by blast
+  from 1 2 step.hyps(1) show ?case by (meson small_step.Seq2 star.simps)
+qed
+
+lemma star_seq_none: 
+  assumes "(Some c1, s) \<rightarrow>* (None, t)"
+  shows "(Some(c1;; c2), s) \<rightarrow>* (Some c2, t)"
+using assms
+proof(induct "(Some c1)" s "None::acom option" t rule: star_induct[where r = small_step])
+  case (step s y s' t)
+  assume 1:"(Some c1, s) \<rightarrow> (y, s')" and 2:"(y, s') \<rightarrow>* (None, t)"
+  have "(Some(c1;; c2), s) \<rightarrow>* (Some c2, t)"
+  proof-
+  {
+    assume 3:"y = None"
+    have "t = s'" using 2 3 none_final(2) by auto
+  (*using 1
+  proof (induct "(Some c1, s)" "(y, s')" rule:small_step.induct)
+    case (Assign P x a)
+    thus ?case using 2 none_final(2) by blast 
+  next
+    case (Seq1 c0 c1')
+    thus ?case*)
+
+qed
+
+lemma seq_comp:
+  "\<lbrakk>(Some c1, s1) \<rightarrow>* (None, s2); (Some c2, s2) \<rightarrow>* (None, s3)\<rbrakk>
+   \<Longrightarrow> (Some (c1;;c2), s1) \<rightarrow>* (None, s3)"
+by(blast intro: star.step star_seq2 star_trans)
 
 end
