Star.thy
@@ -8,16 +8,6 @@ for r where
 refl:  "star r x x" |
 step:  "r x y \<Longrightarrow> star r y z \<Longrightarrow> star r x z"
 
-thm star.induct
-
-lemma star_induct_2:
-  assumes "star r x y"
-  and "\<And> x . P x x" 
-  and "\<And> x y z . \<lbrakk>star r x y; P x y; r y z\<rbrakk> \<Longrightarrow> P x z"
-  shows "P x y"  sorry
-
-hide_fact (open) refl step  --"names too generic"
-
 lemma star_trans:
   "star r x y \<Longrightarrow> star r y z \<Longrightarrow> star r x z"
 proof(induction rule: star.induct)
@@ -25,6 +15,7 @@ proof(induction rule: star.induct)
 next
   case step thus ?case by (metis star.step)
 qed
+
 
 lemmas star_induct =
   star.induct[of "r:: 'a*'b \<Rightarrow> 'a*'b \<Rightarrow> bool", split_format(complete)]
